io/MIO.Behavior.fst
@@ -1,13 +1,13 @@
-module IIO.Behavior
+module MIO.Behavior
 
 open FStar.Ghost
 open FStar.FunctionalExtensionality
 
 open BeyondCriteria
-open IIO
+open MIO
 
 (** Confusing elements:
-1) there are two definitions of trace. one from IIO.Sig.trace and one from BeyondCriteria.trace
+1) there are two definitions of trace. one from MIO.Sig.trace and one from BeyondCriteria.trace
 2) prefixed_trace_property may be confusing 
 **)
 
@@ -16,8 +16,8 @@ about the behavior of contexts. When reasoning about contexts,
 we have to take in account that the context is called by the partial
 program which already produced some events --- that can affect the 
 behavior of the context / the instrumentation **)
-type prefixed_trace_property (pre:IIO.Sig.trace -> Type0) = 
-  h:IIO.Sig.trace -> (#_:squash (pre h)) -> BeyondCriteria.trace #event -> Type0
+type prefixed_trace_property (pre:MIO.Sig.trace -> Type0) = 
+  h:MIO.Sig.trace -> (#_:squash (pre h)) -> BeyondCriteria.trace #event -> Type0
 
 type prefixed_trace (pre:trace->Type0) = h:trace{pre h} * BeyondCriteria.trace #event  
 
@@ -32,29 +32,29 @@ let pt_mem (#pre:trace->Type0) ((h, tr):prefixed_trace pre) (s1:prefixed_trace_p
    'backward predicate transformer 2.3.4' and the 
    'pre-/postcondition transformer 2.3.2' to obtain
    the 'set' of traces produces by the whole program. *)
-val beh_giio : #pre:(trace -> Type0) -> #fl:erased tflag -> dm_giio int fl (to_hist pre (fun _ _ _ -> True)) -> prefixed_trace_property pre 
-let beh_giio ws h tr =
+val beh_gmio : #pre:(trace -> Type0) -> #fl:erased tflag -> dm_gmio int fl (to_hist pre (fun _ _ _ -> True)) -> prefixed_trace_property pre 
+let beh_gmio ws h tr =
   match tr with
   | Infinite_trace _ -> False
   | Finite_trace lt res -> 
-    forall p. dm_giio_theta ws p h ==> p lt res
+    forall p. dm_gmio_theta ws p h ==> p lt res
 
 (* _beh is used on whole programs, thus, 
    we specialize it with the empty history *)
-val _beh : (unit -> IIO int AllActions (fun _ -> True) (fun _ _ _ -> True)) -> trace_property #event
+val _beh : (unit -> MIO int AllActions (fun _ -> True) (fun _ _ _ -> True)) -> trace_property #event
 let _beh ws =
-  beh_giio (reify (ws ())) []
+  beh_gmio (reify (ws ())) []
 
 (** used for whole programs **)
 [@@ "opaque_to_smt"]
-val beh : (unit -> IIO int AllActions (fun _ -> True) (fun _ _ _ -> True)) ^-> trace_property #event
+val beh : (unit -> MIO int AllActions (fun _ -> True) (fun _ _ _ -> True)) ^-> trace_property #event
 let beh = on_domain _ (fun ws -> _beh ws)
 
-val _beh_ctx : #pre:(trace -> Type0) -> (unit -> IIO int AllActions pre (fun _ _ _ -> True)) -> prefixed_trace_property pre 
+val _beh_ctx : #pre:(trace -> Type0) -> (unit -> MIO int AllActions pre (fun _ _ _ -> True)) -> prefixed_trace_property pre 
 let _beh_ctx ws h =
-  beh_giio (reify (ws ())) h
+  beh_gmio (reify (ws ())) h
 
 (** used for contexts **)
 //[@@ "opaque_to_smt"]
-val beh_ctx : #pre:(trace -> Type0) -> (unit -> IIO int AllActions pre (fun _ _ _ -> True)) ^-> prefixed_trace_property pre 
+val beh_ctx : #pre:(trace -> Type0) -> (unit -> MIO int AllActions pre (fun _ _ _ -> True)) ^-> prefixed_trace_property pre 
 let beh_ctx #pre = on_domain _ (fun ws -> _beh_ctx #pre ws)
