io/MIO.fst
@@ -1,11 +1,11 @@
-module IIO
+module MIO
 
 open FStar.Tactics
 open ExtraTactics
 open FStar.Ghost
 
-include IIO.Sig
-open IIO.Sig.Call
+include MIO.Sig
+open MIO.Sig.Call
 open DMFree
 
 (** The postcondition for an io computation is defined over the
@@ -19,31 +19,31 @@ The history is  in reverse chronology order.
 
 At the end of an io computation, the local trace is appended
 in reverse order to the history. **)
-let dm_iio_theta #a = theta #a #iio_cmds #iio_sig #event iio_wps
+let dm_mio_theta #a = theta #a #mio_cmds #mio_sig #event mio_wps
   
-type dm_iio = dm iio_cmds iio_sig event iio_wps
-let dm_iio_return (a:Type) (x:a) : dm_iio a (hist_return x) =
-  dm_return iio_cmds iio_sig event iio_wps a x
+type dm_mio = dm mio_cmds mio_sig event mio_wps
+let dm_mio_return (a:Type) (x:a) : dm_mio a (hist_return x) =
+  dm_return mio_cmds mio_sig event mio_wps a x
 
-val dm_iio_bind  : 
+val dm_mio_bind  : 
   a: Type ->
   b: Type ->
   wp_v: hist a ->
   wp_f: (_: a -> hist b) ->
-  v: dm_iio a wp_v ->
-  f: (x: a -> dm_iio b (wp_f x)) ->
-  Tot (dm_iio b (hist_bind wp_v wp_f))
-let dm_iio_bind a b wp_v wp_f v f = dm_bind iio_cmds iio_sig event iio_wps a b wp_v wp_f v f
+  v: dm_mio a wp_v ->
+  f: (x: a -> dm_mio b (wp_f x)) ->
+  Tot (dm_mio b (hist_bind wp_v wp_f))
+let dm_mio_bind a b wp_v wp_f v f = dm_bind mio_cmds mio_sig event mio_wps a b wp_v wp_f v f
 
-val dm_iio_subcomp : 
+val dm_mio_subcomp : 
   a: Type ->
   wp1: hist a ->
   wp2: hist a ->
-  f: dm_iio a wp1 ->
-  Pure (dm_iio a wp2) (hist_ord wp2 wp1) (fun _ -> True)
-let dm_iio_subcomp a wp1 wp2 f = dm_subcomp iio_cmds iio_sig event iio_wps a wp1 wp2 f
+  f: dm_mio a wp1 ->
+  Pure (dm_mio a wp2) (hist_ord wp2 wp1) (fun _ -> True)
+let dm_mio_subcomp a wp1 wp2 f = dm_subcomp mio_cmds mio_sig event mio_wps a wp1 wp2 f
 
-(** * The IIO effect indexed by actions **)
+(** * The MIO effect indexed by actions **)
 
 (** ** Types **)
 
@@ -51,7 +51,7 @@ let dm_iio_subcomp a wp1 wp2 f = dm_subcomp iio_cmds iio_sig event iio_wps a wp1
 noeq
 type tflag = | NoActions | GetTraceActions | IOActions | AllActions
 
-let rec satisfies (m:iio 'a) (flag:tflag) =
+let rec satisfies (m:mio 'a) (flag:tflag) =
 match flag, m with
 | AllActions,   _                     -> True
 | _,            Return x              -> True
@@ -86,7 +86,7 @@ let (<=) (flag1:tflag) (flag2:tflag) =
 let plus_compat_le (f1 f2 : tflag) : Lemma (f1 <= f1+f2) = ()
 let plus_comm      (f1 f2 : tflag) : Lemma (f1+f2 == f2+f1) = ()
 
-let rec sat_le (f1:tflag) (f2:tflag{f1 <= f2}) (m : iio 'a) :
+let rec sat_le (f1:tflag) (f2:tflag{f1 <= f2}) (m : mio 'a) :
   Lemma (satisfies m f1 ==> satisfies m f2) =
   match m with
   | Return _ -> ()
@@ -97,7 +97,7 @@ let rec sat_le (f1:tflag) (f2:tflag{f1 <= f2}) (m : iio 'a) :
     Classical.forall_intro
      ((fun r -> sat_le f1 f2 (o r)) <: r:_ -> Lemma (satisfies (o r) f1 ==> satisfies (o r) f2))
 
-let rec sat_bind (fl:tflag) (v : iio 'a) (f : 'a -> iio 'b)
+let rec sat_bind (fl:tflag) (v : mio 'a) (f : 'a -> mio 'b)
   : Lemma (v `satisfies` fl /\ (forall x. f x `satisfies` fl) ==> free_bind _ _ _ _ v f `satisfies` fl)
   =
   match v with
@@ -110,13 +110,13 @@ let rec sat_bind (fl:tflag) (v : iio 'a) (f : 'a -> iio 'b)
   Classical.forall_intro
    ((fun r -> sat_bind fl (o r) f) <: r:_ -> Lemma ((o r) `satisfies` fl /\ (forall x. f x `satisfies` fl) ==> free_bind _ _ _ _ (o r) f `satisfies` fl))
 
-let dm_iio_bind_is_free_bind a b wp_v wp_f v f
-: Lemma (dm_iio_bind a b wp_v wp_f v f == free_bind _ _ _ _ v f)
+let dm_mio_bind_is_free_bind a b wp_v wp_f v f
+: Lemma (dm_mio_bind a b wp_v wp_f v f == free_bind _ _ _ _ v f)
 =
-  let r = dm_iio_bind a b wp_v wp_f v f in
+  let r = dm_mio_bind a b wp_v wp_f v f in
   assert (r == free_bind _ _ _ _ v f)
 
-let sat_bind_add (fl_v fl_f:tflag) (v : iio 'a) (f : 'a -> iio 'b)
+let sat_bind_add (fl_v fl_f:tflag) (v : mio 'a) (f : 'a -> mio 'b)
   : Lemma (v `satisfies` fl_v /\ (forall x. f x `satisfies` fl_f) ==> free_bind _ _ _ _ v f `satisfies` (fl_v + fl_f))
   =
   sat_le fl_v (fl_v + fl_f) v;
@@ -128,107 +128,107 @@ let sat_bind_add (fl_v fl_f:tflag) (v : iio 'a) (f : 'a -> iio 'b)
 
 (** ** Defining F* Effect **)
 
-type dm_giio (a:Type) (flag:erased tflag) (wp:hist a) = t:(dm_iio a wp){t `satisfies` flag} 
+type dm_gmio (a:Type) (flag:erased tflag) (wp:hist a) = t:(dm_mio a wp){t `satisfies` flag} 
 
-let dm_giio_theta #a = theta #a #iio_cmds #iio_sig #event iio_wps
+let dm_gmio_theta #a = theta #a #mio_cmds #mio_sig #event mio_wps
 
-let dm_giio_return (a:Type) (x:a) : dm_giio a NoActions (hist_return x) by (compute ()) =
-  dm_iio_return a x
+let dm_gmio_return (a:Type) (x:a) : dm_gmio a NoActions (hist_return x) by (compute ()) =
+  dm_mio_return a x
 
-val dm_giio_bind  : 
+val dm_gmio_bind  : 
   a: Type ->
   b: Type ->
   flag_v : erased tflag ->
   wp_v: Hist.hist a ->
   flag_f : erased tflag ->
   wp_f: (a -> Hist.hist b) ->
-  v: dm_giio a flag_v wp_v ->
-  f: (x: a -> dm_giio b flag_f (wp_f x)) ->
-  Tot (dm_giio b (flag_v + flag_f) (hist_bind wp_v wp_f))
-let dm_giio_bind a b flag_v wp_v flag_f wp_f v f : (dm_giio b (flag_v + flag_f) (hist_bind wp_v wp_f)) =
-  let r = dm_iio_bind a b wp_v wp_f v f in
+  v: dm_gmio a flag_v wp_v ->
+  f: (x: a -> dm_gmio b flag_f (wp_f x)) ->
+  Tot (dm_gmio b (flag_v + flag_f) (hist_bind wp_v wp_f))
+let dm_gmio_bind a b flag_v wp_v flag_f wp_f v f : (dm_gmio b (flag_v + flag_f) (hist_bind wp_v wp_f)) =
+  let r = dm_mio_bind a b wp_v wp_f v f in
   sat_bind_add flag_v flag_f v f;
-  dm_iio_bind_is_free_bind a b wp_v wp_f v f;
+  dm_mio_bind_is_free_bind a b wp_v wp_f v f;
   assert (free_bind _ _ _ _ v f `satisfies` (flag_v + flag_f));
   r
 
-val dm_giio_subcomp : 
+val dm_gmio_subcomp : 
   a: Type ->
   flag1 : erased tflag ->
   wp1: hist a ->
   flag2 : erased tflag ->
   wp2: hist a ->
-  f: dm_giio a flag1 wp1 ->
-  Pure (dm_giio a flag2 wp2) ((flag1 <= flag2) /\ hist_ord wp2 wp1) (fun _ -> True)
-let dm_giio_subcomp a flag1 wp1 flag2 wp2 f =
+  f: dm_gmio a flag1 wp1 ->
+  Pure (dm_gmio a flag2 wp2) ((flag1 <= flag2) /\ hist_ord wp2 wp1) (fun _ -> True)
+let dm_gmio_subcomp a flag1 wp1 flag2 wp2 f =
   sat_le flag1 flag2 f;
-  dm_iio_subcomp a wp1 wp2 f
+  dm_mio_subcomp a wp1 wp2 f
 
-let dm_giio_if_then_else (a : Type u#a)
+let dm_gmio_if_then_else (a : Type u#a)
   (fl1 : erased tflag) (wp1 : hist a)
   (fl2 : erased tflag) (wp2 : hist a)
-  (f : dm_giio a fl1 wp1) (g : dm_giio a fl2 wp2) (b : bool) : Type =
-  dm_giio a (fl1 + fl2) (hist_if_then_else wp1 wp2 b)
+  (f : dm_gmio a fl1 wp1) (g : dm_gmio a fl2 wp2) (b : bool) : Type =
+  dm_gmio a (fl1 + fl2) (hist_if_then_else wp1 wp2 b)
 
 total
 reifiable
 reflectable
 effect {
-  IIOwp (a:Type) (flag:erased tflag) (wp : hist #event a) 
+  MIOwp (a:Type) (flag:erased tflag) (wp : hist #event a) 
   with {
-       repr       = dm_giio
-     ; return     = dm_giio_return
-     ; bind       = dm_giio_bind 
-     ; subcomp    = dm_giio_subcomp
-     ; if_then_else = dm_giio_if_then_else
+       repr       = dm_gmio
+     ; return     = dm_gmio_return
+     ; bind       = dm_gmio_bind 
+     ; subcomp    = dm_gmio_subcomp
+     ; if_then_else = dm_gmio_if_then_else
      }
 }
 
-let dm_giio_partial_return 
-  (pre:pure_pre) : dm_giio (squash pre) NoActions (partial_call_wp pre) by (compute ()) =
-  dm_partial_return iio_cmds iio_sig event iio_wps pre
+let dm_gmio_partial_return 
+  (pre:pure_pre) : dm_gmio (squash pre) NoActions (partial_call_wp pre) by (compute ()) =
+  dm_partial_return mio_cmds mio_sig event mio_wps pre
 
-val lift_pure_dm_giio :
+val lift_pure_dm_gmio :
   a: Type ->
   w: pure_wp a ->
   f: (eqtype_as_type unit -> PURE a w) ->
-  Tot (dm_giio a NoActions (wp_lift_pure_hist w))
-let lift_pure_dm_giio a w f = 
+  Tot (dm_gmio a NoActions (wp_lift_pure_hist w))
+let lift_pure_dm_gmio a w f = 
   lemma_wp_lift_pure_hist_implies_as_requires #a #event w;
   FStar.Monotonic.Pure.elim_pure_wp_monotonicity_forall ();
-  let lhs : dm_giio _ NoActions _ = dm_giio_partial_return (as_requires w) in
-  let rhs = (fun (pre:(squash (as_requires w))) -> dm_giio_return a (f pre)) in
-  let m = dm_giio_bind _ _ NoActions _ NoActions _ lhs rhs in
-  dm_giio_subcomp a NoActions _ NoActions _ m
+  let lhs : dm_gmio _ NoActions _ = dm_gmio_partial_return (as_requires w) in
+  let rhs = (fun (pre:(squash (as_requires w))) -> dm_gmio_return a (f pre)) in
+  let m = dm_gmio_bind _ _ NoActions _ NoActions _ lhs rhs in
+  dm_gmio_subcomp a NoActions _ NoActions _ m
   
-sub_effect PURE ~> IIOwp = lift_pure_dm_giio
+sub_effect PURE ~> MIOwp = lift_pure_dm_gmio
 
-effect IIO
+effect MIO
   (a:Type)
   (fl:erased tflag)
   (pre : trace -> Type0)
   (post : trace -> a -> trace -> Type0) =
-  IIOwp a fl (to_hist pre post) 
+  MIOwp a fl (to_hist pre post) 
   
 let static_cmd
   (isTrusted : bool)
   (cmd : io_cmds)
   (arg : io_sig.args cmd) :
-  IIO (io_sig.res cmd arg) IOActions
+  MIO (io_sig.res cmd arg) IOActions
     (requires (fun h -> io_pre cmd arg h))
     (ensures (fun h (r:io_sig.res cmd arg) lt ->
         lt == [convert_call_to_event isTrusted cmd arg r])) =
-  IIOwp?.reflect (iio_call isTrusted cmd arg)
+  MIOwp?.reflect (mio_call isTrusted cmd arg)
 
-let get_trace (isTrusted:bool) : IIOwp trace GetTraceActions
+let get_trace (isTrusted:bool) : MIOwp trace GetTraceActions
   (fun p h -> p [] h) =
-  IIOwp?.reflect (iio_call isTrusted GetTrace ())
+  MIOwp?.reflect (mio_call isTrusted GetTrace ())
 
 // There is no hope to prove anything about ctx without a meta-theorem about F* / without a formalization of F* & Ghost.
-// val ctx_s : (fl:erased tflag) -> IIO unit fl (fun _ -> True) (fun _ _ _ -> True) 
+// val ctx_s : (fl:erased tflag) -> MIO unit fl (fun _ -> True) (fun _ _ _ -> True) 
 
 private
-let performance_test (#fl:tflag) : IIOwp unit (fl+IOActions) (fun p h -> forall lt. (List.length lt == 6) \/ (List.length lt == 7) ==> p lt ())
+let performance_test (#fl:tflag) : MIOwp unit (fl+IOActions) (fun p h -> forall lt. (List.length lt == 6) \/ (List.length lt == 7) ==> p lt ())
   by (compute ())
 =
   let fd = static_cmd true Openfile "../Makefile" in
