io/MIO.Sig.Call.fst
@@ -1,0 +1,8 @@
+module MIO.Sig.Call
+
+open MIO.Sig
+
+(** This file is replaced during linking with a file that contains the real
+implementation of the commands. **)
+let mio_call (caller:bool) (cmd:cmds) (arg:mio_sig.args cmd) : mio (mio_sig.res cmd arg) =
+  Call caller cmd arg Return
